src/base/wpr_lifting.v
@@ -11,9 +11,9 @@ From self.lang Require Import lang.
 From self.base Require Import generational_resources primitive_laws.
 From self.nextgen Require Import nextgen_promises.
 
-Set Default Proof Using "Type".
+Set Default Proof Using "Type*".
 
-Definition wpr `{!nvmBaseG Σ Ω, !extraStateInterp Σ, !PerennialG Σ}
+Definition wpr `{!nvmBaseGS Σ Ω, !extraStateInterp Σ, !PerennialG Σ}
            (s : stuckness) (E : coPset)
            (e : thread_state) (recv : thread_state) (Φ : thread_val → iProp Σ)
            (Φinv : iProp Σ)
@@ -24,7 +24,7 @@ Definition wpr `{!nvmBaseG Σ Ω, !extraStateInterp Σ, !PerennialG Σ}
     (λ v, Φr v)%I.
 
 Section wpr.
-  Context {Σ : gFunctors} {Ω: gGenCmras Σ}.
+  Context `{!nvmBaseGS Σ Ω, !extraStateInterp Σ, !PerennialG Σ}.
   Implicit Types s : stuckness.
   Implicit Types P : iProp Σ.
   Implicit Types Φ : thread_val → iProp Σ.
@@ -32,7 +32,7 @@ Section wpr.
   Implicit Types v : thread_val.
   Implicit Types e : thread_state.
 
-  Lemma wpr_strong_mono `{!nvmBaseG Σ Ω, !extraStateInterp Σ, !PerennialG Σ}
+  Lemma wpr_strong_mono
         s E e rec Φ Ψ Φinv Ψinv Φr Ψr :
     wpr s E e rec Φ Φinv Φr -∗
     (* TODO: what is this modality? *)
@@ -47,136 +47,14 @@ Section wpr.
     - by iDestruct "Himpl" as "(_ & _ & $)".
   Qed.
 
-  Definition persist_auth `{!nvmBaseG Σ Ω} (σ : mem_config): iProp Σ :=
-    ∃ OCV, persisted_auth (OCV `view_add` σ.2) ∗ crashed_at_offset OCV.
-
-  (* Lemma nvm_heap_reinit σ PV CV `{!nvmBaseG} *)
-  (*       (γcrash : gname) : *)
-  (*   (* The first two assumptions are the content of [crash_step σ σ'] *) *)
-  (*   PV ⊑ CV → *)
-  (*   consistent_cut CV σ → *)
-  (*   valid_heap σ → *)
-  (*   ⊢ gen_heap_interp (hG := _) σ -∗ *)
-  (*     persist_auth (σ, PV) *)
-  (*     ==∗ *)
-  (*     ∃ (hGD' : nvmBaseDeltaG), *)
-  (*       ⌜ @crash_token_name hGD' = γcrash ⌝ ∗ *)
-  (*       validV (hGD := hGD') ∅ ∗ *)
-  (*       post_crash_mapsto_map σ hGD hGD' ∗ *)
-  (*       nvm_heap_ctx (hGD := hGD') (slice_of_store CV σ, view_to_zero CV) ∗ *)
-  (*       persisted_impl hGD hGD' ∗ *)
-  (*       persisted (hGD := hGD') (view_to_zero CV) ∗ *)
-  (*       crashed_at (hGD := hGD') CV. *)
-  (* Proof using Σ. *)
-  (*   iIntros (pIncl cut invs) "heapIntrp pers". *)
-  (*   rewrite /nvm_heap_ctx. simpl. *)
-  (*   (* Allocate a new heap at a _new_ ghost name. *) *)
-  (*   iMod (gen_heap_init_names (slice_of_store CV σ)) as (γh γm) "(heapNew & ptsMap & _)". *)
-  (*   (* We persist/freeze the old persist view. *) *)
-  (*   iMod (own_update with "pers") as "pers". *)
-  (*   { apply auth_update_auth_persist. } *)
-  (*   iDestruct "pers" as "#oldPers". *)
-  (*   (* Allocate a new persist view. *) *)
-  (*   iMod (own_alloc (● (view_to_zero CV) ⋅ ◯ (view_to_zero CV))) as (persistG) "[pers #persFrag]". *)
-  (*   { apply auth_both_valid_2; [apply view_valid|done]. } *)
-  (*   (* Allocate the store view at a _new_ ghost name. *) *)
-  (*   iMod (own_alloc (● max_view (slice_of_store CV σ) ⋅ ◯ ∅)) as (storeG) "[store fragStore]". *)
-  (*   { apply auth_both_valid_2; [apply view_valid | apply: ucmra_unit_least]. } *)
-  (*   (* Allocate the crashed at view at a _new_ ghost name. *) *)
-  (*   iMod (own_alloc (to_agree CV : agreeR viewO)) as (crashedAtG) "#crashed". *)
-  (*   { done. } *)
-  (*   iModIntro. *)
-  (*   set names := {| heap_names_name := Build_nvm_heap_names γh γm; *)
-  (*                   crash_token_name := γcrash; *)
-  (*                   store_view_name := storeG; *)
-  (*                   persist_view_name := persistG; *)
-  (*                   crashed_at_view_name := crashedAtG |}. *)
-  (*   iExists names. *)
-  (*   iSplitPure; first done. *)
-  (*   rewrite /crashed_at_view_name. simpl. *)
-  (*   iFrame. *)
-  (*   iFrame "crashed persFrag". *)
-  (*   (* We show the ghost crash relation. *) *)
-  (*   iSplitL "ptsMap heapIntrp". *)
-  (*   { rewrite /post_crash_mapsto_map. *)
-  (*     iSplitL "heapIntrp". *)
-  (*     { iIntros (???) "pts". *)
-  (*       (* Set Printing All. *) *)
-  (*       iApply (gen_heap_valid with "heapIntrp pts"). } *)
-  (*     iDestruct (big_sepM_impl_strong _ _ _ σ with "ptsMap []") as "[$ _]". *)
-  (*     iModIntro. *)
-  (*     iIntros (ℓ hist) "pts". iIntros (look). *)
-  (*     iApply soft_disj_intro_r. *)
-  (*     iExists _. iFrame "crashed". *)
-  (*     destruct (slice_of_store CV σ !! ℓ) as [?|] eqn:look'; last first. *)
-  (*     * iRight. iPureIntro. *)
-  (*       eapply consistent_cut_lookup_slice; done. *)
-  (*     * iLeft. *)
-  (*       rewrite /slice_of_store /slice_of_hist map_fmap_zip_with in look'. *)
-  (*       rewrite map_fmap_zip_with in look'. *)
-  (*       apply map_lookup_zip_with_Some in look'. *)
-  (*       destruct look' as ([t] & ? & ? & CVLook & ?). *)
-  (*       rewrite /consistent_cut in cut. *)
-  (*       pose proof (map_Forall_lookup_1 _ _ _ _ cut CVLook) as (? & ? & ? & ? & map). *)
-  (*       simplify_eq. *)
-  (*       iExists _, _. *)
-  (*       iSplit; first done. *)
-  (*       rewrite H2. *)
-  (*       rewrite map_fmap_singleton. *)
-  (*       iFrame "pts". *)
-  (*       iPureGoal; first done. *)
-  (*       iPureIntro. *)
-  (*       eapply (map_Forall_lookup_1 _ _ _ _ map). *)
-  (*       rewrite /drop_above. *)
-  (*       apply map_filter_lookup_Some_2; [done| reflexivity]. } *)
-  (*   iSplit. *)
-  (*   * simpl. *)
-  (*     iSplit. { iPureIntro. apply store_inv_cut; done. } *)
-  (*     iExists CV. iFrame "crashed". *)
-  (*     (* TODO: Factor this out into a lemma (needs [cut] only). *) *)
-  (*     apply consistent_cut_subseteq_dom in cut. *)
-  (*     rewrite /slice_of_store /slice_of_hist map_fmap_zip_with. *)
-  (*     rewrite map_fmap_zip_with. *)
-  (*     rewrite dom_map_zip_with_eq_l; try done. *)
-  (*   * iModIntro. *)
-  (*     iIntros (V) "pers". *)
-  (*     rewrite /persisted. *)
-  (*     iDestruct (persisted_auth_included with "oldPers pers") as %incl. *)
-  (*     assert (V ⊑ CV) as incl'. { etrans; done. } *)
-  (*     iSplit. *)
-  (*     { edestruct (view_to_zero_mono) as [? ->]; first apply incl'. *)
-  (*       iDestruct "persFrag" as "[$ _]". } *)
-  (*     iExists CV. iFrame "#%". *)
-  (* Qed. *)
-
-  (* Lemma nvm_heap_reinit_alt σ σ': *)
-  (*   crash_step σ σ' → *)
-  (*   ⊢ nvm_heap_ctx σ -∗ *)
-  (*      |==> ⚡==> |==> *)
-  (*       nvm_heap_ctx (hGD := names) σ' ∗ *)
-  (*       Pg names. *)
-  (* Proof. *)
-  (*   iIntros ([store p p' pIncl cut]). *)
-  (*   iIntros "(heap & authStor & %inv & pers & recov) Pg". *)
-  (*   iMod (nvm_heap_reinit _ _ _ _ _ γcrash with "heap pers") *)
-  (*     as (hGD') "(%crEq & _ & map & interp' & #persImpl & rec)"; try done. *)
-  (*   rewrite /post_crash. *)
-  (*   (* set newBundle : nvmBaseDeltaG := *) *)
-  (*   (*   {| nvmBaseDeltaG' := hnames |}. *) *)
-  (*   iSpecialize ("Pg" $! store hGD'). *)
-  (*   (* rewrite /newBundle. *) *)
-  (*   iDestruct ("Pg" with "persImpl map") as "(map & Pg)". *)
-  (*   iExists _. iModIntro. *)
-  (*   iSplitPure; first done. iFrame. *)
-  (* Qed. *)
-
   (* Is this the only thing I need to prove for high spirea (other than views of course)? *)
-  Lemma extra_state_nextgen `{!nvmBaseG Σ Ω, !extraStateInterp Σ, !PerennialG Σ}:
-    extra_state_interp ⊢ |==> ⚡==> |==> extra_state_interp.
-  Proof.
-  Admitted.
+  Hypothesis extra_state_nextgen: ∀ CV σ1 σ2,
+    CV_crash_step CV σ1 σ2 →
+    extra_state_interp -∗
+    (∃ OCV, crashed_at_offset OCV ∗ picked_out crashed_at_name (crashed_at_trans (OCV `view_add` CV))) -∗
+    |==> ▷ ⚡==> |==> extra_state_interp.
 
-  Lemma idempotence_wpr `{!nvmBaseG Σ Ω, !extraStateInterp Σ, !PerennialG Σ}
+  Lemma idempotence_wpr
       s E1 e e_rec Φ Φinv Φr Φc :
     ⊢ WPC e @ s; E1 {{ Φ }} {{ Φc }} -∗
     (* TODO: have an expert double check this modality *)
@@ -188,22 +66,23 @@ Section wpr.
                             with "[$Hwpc] [Hidemp]").
     (* { iApply (wpc_crash_mono with "[] Hwpc"). *)
     (*   iIntros "HΦcx". iExists _. destruct nG. by iFrame. } *)
-    { iApply (plainly_mono with "[$]").
-      iIntros "Hidemp" (σ_pre_crash g σ_post_crash Hcrash ns mj D κs ?) "ϕc".
-      (* iMod (NC_alloc_strong) as (γcrash) "HNC". *)
-      iSpecialize ("Hidemp" with "ϕc").
-      (* rewrite eq. *)
-      iIntros "[interp extra] g".
-      (* iMod (nvm_heap_reinit_alt _ _ _ _ γcrash _ Hcrash with "interp Hidemp") *)
-      (*   as (hnames) "(%cEq & map & interp' & idemp)". *)
-      iMod (heap_ctx_next_generation _ _ Hcrash with "interp") as "interp".
-      iMod (extra_state_nextgen with "extra") as "extra".
-      do 3 iModIntro. iMod "interp". iMod "extra".
-      iAssert (global_state_interp g (step_count_next ns) mj D κs)%I as "$". { admit. }
-      (* iMod (global_state_interp_le (Λ := nvm_lang) _ _ () _ _ κs with "[$]") as "$"; *)
-      (*   first (rewrite /step_count_next; simpl; lia). *)
-      iModIntro.
-      rewrite /state_interp //=.
-      iFrame.
-  Admitted.
+    iApply (plainly_mono with "[$]").
+    iIntros "Hidemp" (σ_pre_crash g σ_post_crash Hcrash ns mj D κs ?) "ϕc".
+    (* iMod (NC_alloc_strong) as (γcrash) "HNC". *)
+    iSpecialize ("Hidemp" with "ϕc").
+    (* rewrite eq. *)
+    iIntros "[interp extra] g".
+    (* iMod (nvm_heap_reinit_alt _ _ _ _ γcrash _ Hcrash with "interp Hidemp") *)
+    (*   as (hnames) "(%cEq & map & interp' & idemp)". *)
+    destruct Hcrash as [CV Hcrash].
+    iDestruct (heap_ctx_next_generation _ _ _ Hcrash with "interp") as ">[HCV interp]".
+    iDestruct (extra_state_nextgen with "extra HCV") as ">extra"; first done.
+    do 3 iModIntro. iMod "interp". iMod "extra".
+    iAssert (global_state_interp g (step_count_next ns) mj D κs)%I as "$". { by iExistsN. }
+    (* iMod (global_state_interp_le (Λ := nvm_lang) _ _ () _ _ κs with "[$]") as "$"; *)
+    (*   first (rewrite /step_count_next; simpl; lia). *)
+    iModIntro.
+    rewrite /state_interp //=.
+    iFrame.
+  Qed.
 End wpr.
